new simulation that includes a frame (description of
the part of the state that does not change), allows packing environment
relationships into "related" so that we do not need to compose the
simulations under many assumptions any more

compiler/src/compiler/Pipeline.v
@@ -118,6 +118,57 @@ Module Import Pipeline.
 End Pipeline.
 
 
+Section SIM.
+  Context {Frame1 State1: Type}.
+  Context (exec1: State1 -> (State1 -> Prop) -> Prop).
+  Context {Frame2 State2: Type}.
+  Context (exec2: State2 -> (State2 -> Prop) -> Prop).
+  Context (related: Frame1 -> State1 -> Frame2 -> State2 -> Prop).
+
+  Definition simulation := forall f1 f2 (P1: State1 -> Prop) (P2: State2 -> Prop),
+      (forall s1 s2, related f1 s1 f2 s2 -> P1 s1 -> P2 s2) ->
+      forall s1 s2, related f1 s1 f2 s2 -> exec1 s1 P1 -> exec2 s2 P2.
+
+  (* Note: The above could be simplified like this, but then P2 cannot be weakened and we need
+     to carry around a separate hypothesis requiring weakening for language 2. *)
+  Definition simulation_without_weakening := forall (P1: State1 -> Prop) f1 f2 s1 s2,
+      related f1 s1 f2 s2 ->
+      exec1 s1 P1 ->
+      exec2 s2 (fun s2' => exists s1', related f1 s1' f2 s2' /\ P1 s1').
+
+  Definition simulation_alt: simulation -> simulation_without_weakening.
+  Proof. unfold simulation, simulation_without_weakening. eauto 10. Qed.
+
+End SIM.
+
+Section COMPOSE.
+  Context {Frame1 State1: Type}.
+  Context (exec1: State1 -> (State1 -> Prop) -> Prop).
+  Context {Frame2 State2: Type}.
+  Context (exec2: State2 -> (State2 -> Prop) -> Prop).
+  Context {Frame3 State3: Type}.
+  Context (exec3: State3 -> (State3 -> Prop) -> Prop).
+  Context (related12: Frame1 -> State1 -> Frame2 -> State2 -> Prop).
+  Context (related23: Frame2 -> State2 -> Frame3 -> State3 -> Prop).
+
+  Definition compose_related: Frame1 -> State1 -> Frame3 -> State3 -> Prop :=
+    fun f1 s1 f3 s3 => exists f2 s2, related12 f1 s1 f2 s2 /\ related23 f2 s2 f3 s3.
+
+  Lemma compose_simulation(S12: simulation exec1 exec2 related12)(S23: simulation exec2 exec3 related23):
+    simulation exec1 exec3 compose_related.
+  Proof.
+    unfold simulation, compose_related in *.
+    intros f1 f3 P1 P3 P13 s1 s3 (f2 & s2 & HR12 & HR23) Ex1.
+    eapply S23. 2: exact HR23. 2: {
+      eapply S12 with (P2 := (fun s2' => exists s1', related12 f1 s1' f2 s2' /\ P1 s1')).
+      2: exact HR12. 2: exact Ex1. eauto. }
+    intros s2' s3' HR23' (s1' & HR12' & p1). eauto.
+  Qed.
+
+End COMPOSE.
+
+Arguments compose_simulation {_} {_} {_} {_} {_} {_} {_} {_} {_} {_} {_}.
+
 Section Pipeline1.
 
   Context {p: parameters}.
@@ -182,48 +233,191 @@ Section Pipeline1.
     (composePhases spillingPhase
                    (riscvPhase ml)))).
 
-  Section Sim.
-    Context (ml: MemoryLayout)
-            (mlOk: MemoryLayoutOk ml)
-            (f_entry_rel_pos : Z)
-            (f_entry_name : string)
-            (p_call: word) (* address where the call to the entry function is stored *)
-            (p_functions: word) (* address where the compiled functions are stored *)
-            (Rdata Rexec : FlatToRiscvCommon.mem -> Prop)
-            (prog: renamed_env)
-            (e1 : FlattenExpr.ExprImp_env)
-            (e2 : FlattenExpr.FlatImp_env)
-            (funname : string)
-            (Hf: flatten_functions (2 ^ 10) e1 = Some e2).
-    Let c2 := (@FlatImp.SSeq String.string FlatImp.SSkip (FlatImp.SCall [] funname [])).
-    Let c3 := (@FlatImp.SSeq Z FlatImp.SSkip (FlatImp.SCall [] f_entry_name [])).
-    Context (av' : Z) (r' : string_keyed_map Z)
-            (ER: envs_related e2 prog)
-            (Ren: rename map.empty c2 lowest_available_impvar = Some (r', c3, av'))
-            (H_p_call: word.unsigned p_call mod 4 = 0)
-            (H_p_functions: word.unsigned p_functions mod 4 = 0)
-            (G: map.get (FlatToRiscvDef.build_fun_pos_env prog) f_entry_name = Some f_entry_rel_pos)
-            (F: fits_stack 0 (word.unsigned (word.sub (stack_pastend ml) (stack_start ml)) / bytes_per_word) prog
-                           (FlatImp.SSeq FlatImp.SSkip (FlatImp.SCall [] f_entry_name [])))
-            (GEI: good_e_impl prog (FlatToRiscvDef.build_fun_pos_env prog)).
+  Definition FlatState(varname: Type){pp : FlatImp.parameters varname}: Type :=
+    FlatImp.env * FlatImp.stmt varname * bool * FlatImp.trace * FlatImp.mem * FlatImp.locals * MetricLog.
 
-    Definition flattenSim: simulation _ _ _ :=
-      FlattenExprSimulation.flattenExprSim (2^10) e1 e2 funname Hf.
-    Definition regAllocSim: simulation _ _ _ :=
-      renameSim (@ext_spec p)
-                e2 prog c2 c3 av' r' ER Ren.
-    (* Definition spillingSim: simulation _ _ _ *)
-    Definition flatToRiscvSim: simulation _ _ _ :=
-      FlatToRiscvSimulation.flatToRiscvSim
-        f_entry_rel_pos f_entry_name p_call Rdata Rexec
-        p_functions ml.(stack_start) ml.(stack_pastend)
-        prog compile_ext_call_correct H_p_call H_p_functions G F GEI.
+  Definition flatExec{varname: Type}{pp : FlatImp.parameters varname}:
+    FlatState varname -> (FlatState varname -> Prop) -> Prop :=
+    fun '(e, s, done, t, m, l, mc) post =>
+      done = false /\
+      FlatImp.exec e s t m l mc (fun t' m' l' mc' => post (e, s, true, t', m', l', mc')).
 
-    Definition sim: simulation _ _ _ :=
-      (compose_sim flattenSim (compose_sim regAllocSim flatToRiscvSim)).
-  End Sim.
+  Definition flat_related_to_riscv
+             (frame1: @FlatImp.env Z _ * FlatImp.stmt Z)(s1: FlatState Z)
+             (g: GhostConsts)(s2: MetricRiscvMachine): Prop :=
+    let '(e, c, done, t, m, l, mc) := s1 in
+    frame1 = (e, c) /\
+    s2.(getPc) = (if done then word.add g.(p_insts) (word.of_Z (4 * Z.of_nat (length g.(insts))))
+                  else g.(p_insts)) /\
+    e = g.(e_impl) /\
+    good_e_impl g.(e_impl) g.(e_pos) /\
+    fits_stack g.(rem_framewords) g.(rem_stackwords) g.(e_impl) c /\
+    FlatToRiscvDef.stmt_not_too_big c /\
+    FlatToRiscvDef.valid_FlatImp_vars c /\
+    let relpos := (word.unsigned (word.sub g.(p_insts) g.(program_base))) in
+    let stackoffset := (bytes_per_word * g.(rem_framewords)) in
+    FlatToRiscvDef.compile_stmt g.(e_pos) relpos stackoffset c = g.(insts) /\
+    goodMachine t m l g s2.
 
-(*
+  Lemma flatToRiscvSim: simulation flatExec FlatToRiscvCommon.runsTo flat_related_to_riscv.
+  Proof.
+    unfold simulation, flatExec, FlatState, FlatImp.SimExec, flat_related_to_riscv.
+    intros.
+    destruct s1 as ((((((e & c) & done) & t) & m) & l) & mc).
+    destruct_RiscvMachine s2.
+    simp.
+    eapply runsTo_weaken.
+    - specialize compile_stmt_correct with (1 := @compile_ext_call_correct _ h).
+      unfold compiles_FlatToRiscv_correctly. intros compile_stmt_correct.
+      eapply compile_stmt_correct with (g := f2); clear compile_stmt_correct; simpl.
+      + eassumption.
+      + clear. intros k v ?. eassumption.
+      + assumption.
+      + eauto using fits_stack_call.
+      + eassumption.
+      + eassumption.
+      + eassumption.
+      + assert (word.ok word) by exact Utility.word_ok.
+        solve_divisibleBy4.
+        admit.
+      + assert (word.ok word) by exact Utility.word_ok.
+        solve_divisibleBy4.
+        admit.
+      + (* TODO why are these manual steps needed? *)
+        admit.
+      + assert (word.ok word) by exact Utility.word_ok.
+        admit.
+      + assumption.
+    - simpl. intros. simp.
+      eapply H. 2: eassumption.
+      cbv beta iota.
+      repeat match goal with
+             | |- _ /\ _ => split
+             | _ => eassumption
+             | _ => reflexivity
+             end.
+      all: fail.
+  Admitted.
+
+  Definition spilling_related
+             (frame1: @FlatImp.env Z _ * FlatImp.stmt Z)(s1: FlatState Z)
+             (frame2: @FlatImp.env Z _ * FlatImp.stmt Z)(s2: FlatState Z) :=
+    let '(e1, c1, done1, t1, m1, l1, mc1) := s1 in
+    let '(e2, c2, done2, t2, m2, l2, mc2) := s2 in
+    frame1 = (e1, c1) /\
+    frame2 = (e2, c2) /\
+    done1 = done2 /\
+    c2 = spill_stmt c1 /\
+    exists maxvar (fpval: word),
+      Spilling.envs_related e1 e2 /\
+      Spilling.valid_vars_src maxvar c1 /\
+      Spilling.related ext_spec maxvar (emp True) fpval t1 m1 l1 t2 m2 l2.
+
+  Lemma spilling_sim: simulation flatExec flatExec spilling_related.
+  Proof.
+    unfold simulation, flatExec, spilling_related. intros f1 f2 P1 P2 R.
+    intros ((((((e1 & c1) & done1) & t1) & m1) & l1) & mc1) ((((((e2 & c2) & done2) & t2) & m2) & l2) & mc2).
+    intros. simp. split; [reflexivity|].
+    eapply FlatImp.exec.weaken.
+    - eapply spilling_correct; eassumption.
+    - cbv beta. intros. simp. eapply R. 2: eassumption. simpl.
+      eauto 10.
+  Qed.
+
+  Definition renaming_related
+             (frame1: @FlatImp.env string _ * FlatImp.stmt string)(s1: FlatState string)
+             (frame2: @FlatImp.env Z _ * FlatImp.stmt Z)(s2: FlatState Z) :=
+    let '(e1, c1, done1, t1, m1, l1, mc1) := s1 in
+    let '(e2, c2, done2, t2, m2, l2, mc2) := s2 in
+    frame1 = (e1, c1) /\
+    frame2 = (e2, c2) /\
+    done1 = done2 /\
+    RegRename.envs_related e1 e2 /\
+    (exists r' av', RegRename.rename map.empty c1 lowest_available_impvar = Some (r', c2, av')) /\
+    t1 = t2 /\
+    m1 = m2 /\
+    (done1 = false -> l1 = map.empty /\ l2 = map.empty /\ mc1 = mc2).
+
+  Lemma renaming_sim: simulation flatExec flatExec renaming_related.
+  Proof.
+    unfold simulation, flatExec, renaming_related. intros f1 f2 P1 P2 R.
+    intros ((((((e1 & c1) & done1) & t1) & m1) & l1) & mc1) ((((((e2 & c2) & done2) & t2) & m2) & l2) & mc2).
+    intros. simp. split; [reflexivity|]. specialize (Hp3 eq_refl). simp.
+    pose proof Hp1 as A.
+    apply rename_props in A;
+      [|eapply map.empty_injective|eapply dom_bound_empty].
+    simp.
+    eapply FlatImp.exec.weaken.
+    - eapply rename_correct.
+      1: eassumption.
+      1: eassumption.
+      3: {
+        eapply Ap2. eapply TestLemmas.extends_refl.
+      }
+      1: eassumption.
+      1: eassumption.
+      unfold states_compat. intros *. intro B.
+      erewrite map.get_empty in B. discriminate.
+    - simpl. intros. simp.
+      eapply R. 2: eassumption. simpl. clear R. intuition (discriminate || eauto).
+  Qed.
+
+  Definition SrcState: Type :=
+    Semantics.env * Syntax.cmd * bool * Semantics.trace * Semantics.mem * Semantics.locals * MetricLog.
+
+  Definition srcExec: SrcState -> (SrcState -> Prop) -> Prop :=
+    fun '(e, c, done, t, m, l, mc) post =>
+      done = false /\
+      Semantics.exec e c t m l mc (fun t' m' l' mc' => post (e, c, true, t', m', l', mc')).
+
+  Definition flattening_related
+             (frame1: Semantics.env * Syntax.cmd)(s1: SrcState)
+             (frame2: @FlatImp.env string _ * FlatImp.stmt string)(s2: FlatState string) :=
+    let '(e1, c1, done1, t1, m1, l1, mc1) := s1 in
+    let '(e2, c2, done2, t2, m2, l2, mc2) := s2 in
+    frame1 = (e1, c1) /\
+    frame2 = (e2, c2) /\
+    done1 = done2 /\
+    (exists ngs', flattenStmt (freshNameGenState (ExprImp.allVars_cmd_as_list c1)) c1 = (c2, ngs')) /\
+    flatten_functions (2^10) e1 = Some e2 /\
+    t1 = t2 /\
+    m1 = m2 /\
+    (done1 = false -> l1 = map.empty /\ l2 = map.empty /\ mc1 = mc2).
+
+  Lemma flattening_sim: simulation srcExec flatExec flattening_related.
+  Proof.
+    unfold simulation, srcExec, flatExec, flattening_related. intros f1 f2 P1 P2 R.
+    intros ((((((e1 & c1) & done1) & t1) & m1) & l1) & mc1) ((((((e2 & c2) & done2) & t2) & m2) & l2) & mc2).
+    intros. simp. split; [reflexivity|]. specialize (Hp3 eq_refl). simp.
+    eapply FlatImp.exec.weaken.
+    - eapply @flattenStmt_correct_aux with (eH := e1).
+      + typeclasses eauto.
+      + eassumption.
+      + eassumption.
+      + reflexivity.
+      + eassumption.
+      + intros x k A. rewrite map.get_empty in A. discriminate.
+      + unfold map.undef_on, map.agree_on. intros. reflexivity.
+      + eapply freshNameGenState_disjoint.
+    - simpl. intros. simp. eapply R. 2: eassumption. simpl. intuition (discriminate || eauto).
+  Qed.
+
+  Definition related: Semantics.env * Syntax.cmd -> SrcState -> GhostConsts -> MetricRiscvMachine -> Prop :=
+    (compose_related flattening_related
+    (compose_related renaming_related
+    (compose_related spilling_related
+                     flat_related_to_riscv))).
+
+  Lemma sim: simulation srcExec FlatToRiscvCommon.runsTo related.
+  Proof.
+    exact (compose_simulation flattening_sim
+          (compose_simulation renaming_sim
+          (compose_simulation spilling_sim
+                              flatToRiscvSim))).
+  Qed.
+
+  Axiom TODO: False.
+
   Lemma rename_fun_valid: forall argnames retnames body impl',
       rename_fun (argnames, retnames, body) = Some impl' ->
       NoDup argnames ->
@@ -247,6 +441,8 @@ Section Pipeline1.
     { assumption. }
     { assumption. }
     simp.
+    set (lowest_nonregister := 32).
+    assert (Z.leb z1 lowest_nonregister = true) as E2 by case TODO.
     ssplit.
     - eapply Forall_impl. 2: {
         eapply map.getmany_of_list_in_map. eassumption.
@@ -609,6 +805,50 @@ Section Pipeline1.
       (* configured by PrimitivesParams, can contain invariants needed for external calls *)
       valid_machine mach.
 
+  Lemma establish_undone_related: forall
+      (ml: MemoryLayout)
+      (mlOk: MemoryLayoutOk ml)
+      (f_entry_name : string) (fbody: Syntax.cmd.cmd) (f_entry_rel_pos: Z)
+      (p_call p_functions: word)
+      (Rdata Rexec : mem -> Prop)
+      (functions: source_env)
+      (instrs: list Instruction)
+      (pos_map: funname_env Z)
+      (mH: mem) (mc: MetricLog)
+      (initial: MetricRiscvMachine),
+      ExprImp.valid_funs functions ->
+      compile ml functions = Some (instrs, pos_map) ->
+      map.get functions f_entry_name = Some (nil, nil, fbody) ->
+      map.get pos_map f_entry_name = Some f_entry_rel_pos ->
+      machine_ok p_functions f_entry_rel_pos ml.(stack_start) ml.(stack_pastend) instrs
+                 p_call p_call mH Rdata Rexec initial ->
+      exists riscv_frame,
+        related (functions, fbody) (functions, fbody, false, getLog initial, mH, map.empty, mc)
+                riscv_frame initial.
+  Proof.
+
+  Admitted.
+
+  Lemma done_related_to_machine_ok: forall
+      (ml: MemoryLayout)
+      (mlOk: MemoryLayoutOk ml)
+      (fbody: Syntax.cmd.cmd) (f_entry_rel_pos: Z)
+      (p_call p_functions: word)
+      (Rdata Rexec : mem -> Prop)
+      (functions: source_env)
+      (instrs: list Instruction)
+      (t: Semantics.trace) (lH: Semantics.locals) (mH: mem) (mc: MetricLog)
+      (mach: MetricRiscvMachine)
+      (riscv_frame: GhostConsts),
+      related (functions, fbody) (functions, fbody, true, t, mH, lH, mc)
+              riscv_frame mach ->
+      machine_ok p_functions f_entry_rel_pos ml.(stack_start) ml.(stack_pastend) instrs
+                 p_call (word.add p_call (word.of_Z 4)) mH Rdata Rexec mach /\
+      t = mach.(getLog).
+  Proof.
+
+  Admitted.
+
   (* This lemma translates "sim", which depends on the large definition "related", into something
      more understandable and usable. *)
   Lemma compiler_correct: forall
@@ -636,27 +876,107 @@ Section Pipeline1.
                      p_call (word.add p_call (word.of_Z 4)) mH' Rdata Rexec final).
   Proof.
     intros.
+    edestruct establish_undone_related as (g & R); [eassumption..|].
+    eapply runsTo_weaken.
+    - pose proof sim as P. eapply simulation_alt in P.
+      unfold simulation_without_weakening, SrcState, srcExec in P.
+      let x := open_constr:((_, _, _, _, _, _, _):
+        Semantics.env * Syntax.cmd.cmd * bool * Semantics.trace * Semantics.mem * Semantics.locals * MetricLog)
+      in specialize P with (s1 := x).
+      let x := open_constr:((_, _): Semantics.env * Syntax.cmd.cmd)
+      in specialize P with (f1 := x).
+      specialize P with (P1 := fun '(e', c', done', t', m', l', mc') =>
+                                 e' = functions /\ c' = fbody /\ done' = true /\ postH t' m').
+      simpl in P.
+      eapply P; clear P. 1: exact R.
+      split; [reflexivity|]. eapply ExprImp.weaken_exec. 1: eassumption.
+      cbv beta. eauto.
+    - cbv beta. intros final A. simp.
+      edestruct done_related_to_machine_ok as (A & ?). 1: exact mlOk. 1: exact Ap0. subst t.
+      eauto.
+  Qed.
+
+  (* Old proof: *)
+  Goal forall
+      (ml: MemoryLayout)
+      (mlOk: MemoryLayoutOk ml)
+      (f_entry_name : string) (fbody: Syntax.cmd.cmd) (f_entry_rel_pos: Z)
+      (p_call p_functions: word)
+      (Rdata Rexec : mem -> Prop)
+      (functions: source_env)
+      (instrs: list Instruction)
+      (pos_map: funname_env Z)
+      (mH: mem) (mc: MetricLog)
+      (postH: Semantics.trace -> Semantics.mem -> Prop)
+      (initial: MetricRiscvMachine),
+      ExprImp.valid_funs functions ->
+      compile ml functions = Some (instrs, pos_map) ->
+      map.get functions f_entry_name = Some (nil, nil, fbody) ->
+      map.get pos_map f_entry_name = Some f_entry_rel_pos ->
+      Semantics.exec functions fbody initial.(getLog) mH map.empty mc (fun t' m' l' mc' => postH t' m') ->
+      machine_ok p_functions f_entry_rel_pos ml.(stack_start) ml.(stack_pastend) instrs
+                 p_call p_call mH Rdata Rexec initial ->
+      runsTo initial (fun final => exists mH',
+          postH final.(getLog) mH' /\
+          machine_ok p_functions f_entry_rel_pos ml.(stack_start) ml.(stack_pastend) instrs
+                     p_call (word.add p_call (word.of_Z 4)) mH' Rdata Rexec final).
+  Proof.
+    intros.
     match goal with
     | H: map.get pos_map _ = Some _ |- _ => rename H into GetPos
     end.
-    unfold compile, composePhases, renamePhase, flattenPhase in *. simp.
+    unfold compile, composePhases, flattenPhase, renamePhase, spillingPhase in *. simp.
+
+    match goal with
+    | H: flatten_functions _ _ = _ |- _ => rename H into FlattenEq
+    end.
+    unfold flatten_functions in FlattenEq.
+    match goal with
+    | H: _ |- _ => unshelve epose proof (map.map_all_values_fw _ _ _ _ FlattenEq _ _ H)
+    end.
+    simp.
+    match goal with
+    | H: rename_functions _ = _ |- _ => rename H into RenameEq
+    end.
+    unfold rename_functions in RenameEq.
+    match goal with
+    | H: _ |- _ => unshelve epose proof (map.map_all_values_fw _ _ _ _ RenameEq _ _ H)
+    end.
+    simp.
+    match goal with
+    | H: flatten_function _ _ = _ |- _ => rename H into FF
+    end.
+    unfold flatten_function in FF. simp.
+
     eapply runsTo_weaken.
-    - pose proof sim as P. unfold simulation, ExprImp.SimState, ExprImp.SimExec in P.
-      specialize (P ml f_entry_rel_pos f_entry_name p_call p_functions Rdata Rexec).
-      specialize P with (e1 := functions) (s1 := (initial.(getLog), mH, map.empty, mc)).
-      specialize P with (post1 := fun '(t', m', l', mc') => postH t' m').
+    - pose proof sim as P. eapply simulation_alt in P.
+      unfold simulation_without_weakening, SrcState, srcExec in P.
+      let x := open_constr:((_, _, _, _, _, _, _):
+        Semantics.env * Syntax.cmd.cmd * bool * Semantics.trace * Semantics.mem * Semantics.locals * MetricLog)
+      in specialize P with (s1 := x).
+      let x := open_constr:((_, _): Semantics.env * Syntax.cmd.cmd)
+      in specialize P with (f1 := x).
+      specialize P with (P1 := fun '(e', c', done', t', m', l', mc') =>
+                                 e' = functions /\ c' = fbody /\ done' = true /\ postH t' m').
       simpl in P.
-      eapply P; clear P; cycle -1. {
-        econstructor.
-        + eassumption.
-        + reflexivity.
-        + unfold map.of_list_zip, map.putmany_of_list_zip. reflexivity.
-        + eassumption.
-        + intros. exists nil. split; [reflexivity|].
-          exists map.empty. split; [reflexivity|].
-          eassumption.
+      eapply P; clear P. 2: {
+        split; [reflexivity|]. eapply ExprImp.weaken_exec. 1: eassumption.
+        cbv beta. eauto.
       }
-      { eassumption. }
+      unfold related, flattening_related, renaming_related, spilling_related, flat_related_to_riscv,
+             compose_related.
+      eexists (_, _), (_, _, _, _, _, _, _).
+      ssplit; try reflexivity; eauto.
+      { eexists.
+        match goal with
+        | |- ?x = (?evar1, ?evar2) => transitivity (fst x, snd x)
+        end.
+        2: reflexivity.
+        match goal with
+        | |- ?x = (_, _) => destruct x; reflexivity
+        end. }
+      eexists (_, _), (_, _, _, _, _, _, _).
+      ssplit; try reflexivity; eauto.
       { unfold envs_related.
         intros f [ [argnames resnames] body1 ] G.
         unfold rename_functions in *.
@@ -664,85 +984,10 @@ Section Pipeline1.
         5: exact G. 4: eassumption.
         - eapply String.eqb_spec.
         - typeclasses eauto.
-        - typeclasses eauto.
+        - simpl. typeclasses eauto.
       }
-      { reflexivity. }
-      { unfold machine_ok in *. simp. solve_divisibleBy4. }
-      { unfold riscvPhase, machine_ok in *. simp.
-        eapply program_mod_4_0. 2: ecancel_assumption.
-        destruct (map.map_all_values_fw _ _ _ _ E _ _ H1) as [ [ [args' rets'] fbody' ] [ F G ] ].
-        unfold flatten_function in F. simp.
-        epose proof (map.map_all_values_fw _ _ _ _ E0 _ _ G) as [ [ [args' rets'] fbody' ] [ F G' ] ].
-        unfold rename_fun in F. simp.
-        eapply compile_funs_nonnil; eassumption.
-      }
-      { unfold riscvPhase in *. simp. exact GetPos. }
-      { simpl. unfold riscvPhase in *. simpl in *. simp.
-        move E1 at bottom.
-        eapply fits_stack_seq. 1: eapply fits_stack_skip. 1: reflexivity. {
-          eapply Z.div_pos.
-          - eapply proj1. eapply word.unsigned_range.
-          - clear. unfold bytes_per_word, Memory.bytes_per.
-            destruct width_cases as [E | E]; rewrite E; reflexivity.
-        }
-        destruct (map.map_all_values_fw _ _ _ _ E _ _ H1) as [ [ [args' rets'] fbody' ] [ F G ] ].
-        unfold flatten_function in F. simp.
-        epose proof (map.map_all_values_fw _ _ _ _ E0 _ _ G) as [ [ [args' rets'] fbody' ] [ F G' ] ].
-        unfold rename_fun in F. simp.
-        apply_in_hyps rename_binds_preserves_length.
-        destruct rets'; [|discriminate].
-        destruct args'; [|discriminate].
-        repeat match goal with
-               | H: _ |- _ => autoforward with typeclass_instances in H
-               end.
-        econstructor. 1: reflexivity. 1: eassumption.
-        eapply fits_stack_monotone.
-        1: eapply stack_usage_correct; eassumption. 1: reflexivity. blia. }
-      { unfold good_e_impl.
-        intros.
-        simpl in *.
-        match goal with
-        | H: rename_functions _ = _ |- _ => rename H into RenameEq
-        end.
-        unfold rename_functions in RenameEq.
-        match goal with
-        | H: _ |- _ => unshelve epose proof (map.map_all_values_bw _ _ _ _ RenameEq _ _ H)
-        end.
-        simp. destruct v1 as [ [argnames' retnames'] body' ].
-        match goal with
-        | H: flatten_functions _ _ = _ |- _ => rename H into FlattenEq
-        end.
-        unfold flatten_functions in FlattenEq.
-        match goal with
-        | H: _ |- _ => unshelve epose proof (map.map_all_values_bw _ _ _ _ FlattenEq _ _ H) as P
-        end.
-        unfold flatten_function in P.
-        simp.
-        match goal with
-        | H: ExprImp.valid_funs _ |- _ => rename H into V
-        end.
-        unfold ExprImp.valid_funs in V.
-        specialize V with (1 := Pp1).
-        unfold ExprImp.valid_fun in V.
-        destruct V.
-        ssplit.
-        - eapply rename_fun_valid; try eassumption.
-          unfold ExprImp2FlatImp in *.
-          simp.
-          repeat match goal with
-                 | H: @eq bool _ _ |- _ => autoforward with typeclass_instances in H
-                 end.
-          assumption.
-        - unfold FlatToRiscvDef.build_fun_pos_env, FlatToRiscvDef.build_fun_pos_env.
-          pose proof (get_compile_funs_pos r0) as P.
-          destruct (FlatToRiscvDef.compile_funs map.empty r0) as [ insts posmap ] eqn: F.
-          eapply P.
-          eassumption.
-      }
-      unfold related, compose_relation.
-      unfold FlatToRiscvSimulation.related, FlattenExprSimulation.related, RegRename.related.
-      refine (ex_intro _ (_, _, _, _) _).
-      ssplit; try reflexivity.
+      all: admit.
+      (*
       refine (ex_intro _ (_, _, _, _) _).
       ssplit; try reflexivity.
       { intros. ssplit; reflexivity. }
@@ -812,7 +1057,8 @@ Section Pipeline1.
         apply Hlength_stack_trash_words. }
       { reflexivity. }
       { unfold machine_ok in *. simp. assumption. }
-    - intros. unfold compile_inv, related, compose_relation in *.
+      *)
+    - intros. unfold compile_inv, related, compose_related in *.
       match goal with
       | H: context[machine_ok] |- _ =>
         unfold machine_ok in H;
@@ -829,7 +1075,10 @@ Section Pipeline1.
       repeat match goal with
              | H: context[Semantics.exec] |- _ => clear H
              end.
+      unfold flattening_related, renaming_related, spilling_related, flat_related_to_riscv in *.
       unfold FlatToRiscvSimulation.related, FlattenExprSimulation.related, RegRename.related, goodMachine in *.
+      admit.
+      (*
       simp.
       eexists. split. 1: eassumption.
       unfold machine_ok. ssplit; try assumption.
@@ -903,6 +1152,7 @@ Section Pipeline1.
         simpl.
         wwcancel.
       + destr_RiscvMachine final. subst. solve_divisibleBy4.
+      *)
     Unshelve.
     all: try exact (bedrock2.MetricLogging.mkMetricLog 0 0 0 0).
     all: try (simpl; typeclasses eauto).
@@ -910,8 +1160,7 @@ Section Pipeline1.
     all: try exact nil.
     all: try exact map.empty.
     all: try exact mem_ok.
-  Qed.
-*)
+  Abort.
 
   Definition instrencode(p: list Instruction): list byte :=
     List.flat_map (fun inst => HList.tuple.to_list (LittleEndian.split 4 (encode inst))) p.
